cleanup eq_dist

Iris/Iris/Algebra/OFE.lean
@@ -36,8 +36,13 @@ open OFE
 
 scoped notation:40 x " ≡{" n "}≡ " y:41 => OFE.Dist n x y (SI := stepindex%)
 
-abbrev OFE.eq_dist (SI := by infer_stepindex) [SIdx SI] {α} [self : IOFE SI α] {x y : α} :
+theorem OFE.eq_dist {SI} [SIdx SI] {α} [self : IOFE SI α] {x y : α} :
   x = y ↔ ∀ n, OFE.Dist (SI:=SI) n x y := OFE.eq_dist'
+
+theorem OFE.eq_dist_1 {SI} [SIdx SI] {α} [self : IOFE SI α] {x y : α} :
+  x = y → ∀ n, OFE.Dist (SI:=SI) n x y := OFE.eq_dist.mp
+theorem OFE.eq_dist_2 {SI} [SIdx SI] {α} [self : IOFE SI α] {x y : α} :
+  (∀ n, OFE.Dist (SI:=SI) n x y) → x = y := OFE.eq_dist.mpr
 
 namespace OFE
 
@@ -138,7 +143,7 @@ theorem distLater_succ [OFE α] {n : SI} {x y : α} : DistLater (SIdx.succ n) x 
   ⟨(·.dist_lt (SIdx.lt_succ_self _)), fun h1 _ h2 => h1.le (SIdx.lt_succ_r.mp h2)⟩
 
 theorem distLater_soundness [OFE α] {x y : α} (H : ∀ n, DistLater n x y → x ≡{n}≡ y) : x = y := by
-  refine (eq_dist ..).mpr fun (n : SI) => ?_
+  refine eq_dist_2 fun (n : SI) => ?_
   induction n using instSI.lt_wf.induction with
   | _ n IH => exact H n IH
 
@@ -390,7 +395,7 @@ instance : @DiscreteE SI _ Unit unitOFE (() : Unit) :=
 instance [OFE α] : OFE (ULift α) where
   Dist n x y := x.down ≡{n}≡ y.down
   dist_eqv := InvImage.equivalence dist_eqv
-  eq_dist' {x y} := by cases x; cases y; rw [ULift.up.injEq]; exact (eq_dist _)
+  eq_dist' {x y} := by cases x; cases y; rw [ULift.up.injEq]; exact eq_dist
   dist_lt := dist_lt
 
 def uliftUpHom [OFE α] : α -n> ULift α where
@@ -509,7 +514,7 @@ instance [OFEFun (SI := SI) (β : α → _)] : OFE ((x : α) → β x) where
     symm h _ := dist_eqv.symm (h _)
     trans h1 h2 _ := dist_eqv.trans (h1 _) (h2 _)
   }
-  eq_dist' {_ _} := by rw [funext_iff]; simpa only [eq_dist _] using forall_comm
+  eq_dist' {_ _} := by rw [funext_iff]; simpa only [eq_dist (SI:=_)] using forall_comm
   dist_lt h1 h2 _ := dist_lt (h1 _) h2
 #rocq_ignore discrete_funO "Use a function type"
 #rocq_ignore discrete_fun "Lean uses `(x : α) → β x` directly with `OFEFun`."
@@ -585,7 +590,7 @@ instance [OFE α] [OFE β] : OFE (α × β) where
     symm h := ⟨dist_eqv.symm h.1, dist_eqv.symm h.2⟩
     trans h1 h2 := ⟨dist_eqv.trans h1.1 h2.1, dist_eqv.trans h1.2 h2.2⟩
   }
-  eq_dist' {_ _} := by rw [Prod.ext_iff]; simp only [eq_dist _, forall_and]
+  eq_dist' {_ _} := by rw [Prod.ext_iff]; simp only [eq_dist (SI:=_), forall_and]
   dist_lt h1 h2 := ⟨dist_lt h1.1 h2, dist_lt h1.2 h2⟩
 #rocq_ignore prodO "Use product type"
 #rocq_ignore prod_dist "Implicit in Prod OFE"
@@ -671,8 +676,8 @@ instance : OFE (α ⊕ β) where
   }
   eq_dist' {a b} := by
     match a, b with
-    | .inl _, .inl _ => rw [Sum.inl.injEq]; exact eq_dist _
-    | .inr _, .inr _ => rw [Sum.inr.injEq]; exact eq_dist _
+    | .inl _, .inl _ => rw [Sum.inl.injEq]; exact eq_dist
+    | .inr _, .inr _ => rw [Sum.inr.injEq]; exact eq_dist
     | .inl _, .inr _ => exact ⟨fun h => (nomatch h), fun x => (x 0).elim⟩
     | .inr _, .inl _ => exact ⟨fun h => (nomatch h), fun x => (x 0).elim⟩
   dist_lt {_ a b} := match a, b with
@@ -778,7 +783,7 @@ instance instOFESigma (P : α → Type _) [∀ x, OFE (P x)] : OFE (Sigma P) whe
     obtain ⟨heq, _⟩ := h 0
     obtain ⟨xf, xs⟩ := x; obtain ⟨yf, ys⟩ := y
     simp only at heq; subst heq
-    exact congrArg _ ((eq_dist _).mpr fun n => (h n).2)
+    exact congrArg _ (eq_dist_2 fun n => (h n).2)
   dist_lt {_ x y} := match x, y with
     | ⟨x, xH⟩, ⟨y, yH⟩ => fun
       | ⟨heq, H⟩ => fun hlt => ⟨heq, by simp only at heq; subst heq; exact dist_lt H hlt⟩
@@ -1066,13 +1071,13 @@ theorem conv_compl' [COFE α] {c : Chain α} {n i} (h : n ≤ i) : compl c ≡{n
 @[rocq_alias compl_chain_map]
 theorem compl_map [COFE α] [COFE β] (f : α -n> β) (c : Chain α) :
     compl (Chain.map f c) = f (compl c) := by
-  refine (OFE.eq_dist _).mpr (fun (n : SI) => ?_)
+  refine OFE.eq_dist_2 (fun (n : SI) => ?_)
   exact Dist.trans conv_compl (NonExpansive.ne (Dist.symm conv_compl))
 
 /-- Constant chains complete to their constant value -/
 @[simp, rocq_alias compl_chain_const]
 theorem compl_const [COFE α] (a : α) : compl (Chain.const a) = a :=
-  (OFE.eq_dist _).mpr (fun _ => conv_compl)
+  OFE.eq_dist_2 (fun _ => conv_compl)
 
 /-- Completion of discrete COFEs is the constant value. -/
 @[simp] theorem discrete_cofe_compl [COFE α] [OFE.Discrete α] (c : Chain α) : compl c = c 0 :=
@@ -1731,8 +1736,8 @@ instance instOFunctorHomOF [OFunctor F1] [OFunctor F2] : OFunctor (HomOF F1 F2) 
   ofe := inferInstance
   map f g := Hom.map (map (F := F1) g f) (map (F := F2) f g)
   map_ne.ne _ _ _ Hf _ _ Hg := NonExpansive₂.ne (map_ne.ne Hg Hf) (map_ne.ne Hf Hg)
-  map_id x := (OFE.eq_dist _).mpr fun _ a => ((map_id _).trans (congrArg x.f (map_id a))).dist
-  map_comp _ _ _ _ x := (OFE.eq_dist _).mpr fun _ _ =>
+  map_id x := OFE.eq_dist_2 fun _ a => ((map_id _).trans (congrArg x.f (map_id a))).dist
+  map_comp _ _ _ _ x := OFE.eq_dist_2 fun _ _ =>
     ((map_comp _ _ _ _ _).trans (congrArg _ (congrArg _ (congrArg x.f (map_comp _ _ _ _ _))))).dist
 
 open OFunctorContractive in
@@ -1812,7 +1817,7 @@ theorem LimitPreserving.equiv [SIdxFinite SI] [COFE α] [COFE β] (f g : α -n> 
     LimitPreserving (fun x => f x = g x) := by
   apply of_sidx_finite.mp
   intro c Hfg
-  refine (eq_dist _).mpr fun n => ?_
+  refine eq_dist_2 fun n => ?_
   apply (COFE.compl_map _ _).symm.dist.trans
   apply (COFE.conv_compl' SIdx.le_refl).trans
   apply (Hfg _).dist.trans
@@ -1927,7 +1932,7 @@ def fixpointAux [COFE α] [Inhabited α] (f : α → α) [Contractive f] : α :=
 
 theorem fixpointAux_unfold [COFE α] [Inhabited α] (f : α -c> α) :
     fixpointAux f = f (fixpointAux f) := by
-  refine (eq_dist _).mpr fun (n : SI) => ?_
+  refine eq_dist_2 fun (n : SI) => ?_
   apply COFE.conv_compl.trans
   refine .trans ?_ (NonExpansive.ne COFE.conv_compl.symm)
   exact Contractive.distLater_dist fun p Hp => ((fixpointBFChain f.f n).fixpoint p Hp).symm
@@ -1956,7 +1961,7 @@ theorem fixpoint_unfold [COFE α] [Inhabited α] (f : α -c> α) :
 @[rocq_alias fixpoint_unique]
 theorem fixpoint_unique [COFE α] [Inhabited α] {f : α -c> α} {x : α} (h : x = f x) :
     x = fixpoint f := by
-  refine (eq_dist _).mpr fun (n : SI) => ?_
+  refine eq_dist_2 fun (n : SI) => ?_
   induction n using instSI.lt_wf.induction with
   | h n ih =>
     exact h.dist.trans <| Dist.trans (Contractive.distLater_dist ih) (fixpoint_unfold f).dist.symm
@@ -2119,7 +2124,7 @@ instance isOFE_later [OFE A] : OFE (Later A) where
   dist_eqv := ⟨fun _ => .rfl, .symm, .trans⟩
   eq_dist' {x y} := by
     obtain ⟨a⟩ := x; obtain ⟨b⟩ := y
-    simp only [Later.next.injEq, eq_dist _]
+    simp only [Later.next.injEq, eq_dist (SI:=_)]
     exact ⟨fun H n => (H n).distLater, fun H n => (H (SIdx.succ n)).dist_lt (SIdx.lt_succ_self n)⟩
   dist_lt Hxy Hmn _ Hkm := Hxy _ (SIdx.lt_trans Hkm Hmn)
 #rocq_ignore laterO "Use the later type"
