Iris/Iris/Algebra/CMRA.lean
@@ -718,7 +718,7 @@ variable {α : Type _} [CMRA α]
 
 @[rocq_alias cancelable]
 theorem cancelable {x y z : α} [Cancelable x] (v : ✓(x • y)) (e : x • y = x • z) : y = z :=
-  (OFE.eq_dist _).mpr fun _ => cancelableN v.validN e.dist
+  OFE.eq_dist_2 fun _ => cancelableN v.validN e.dist
 
 @[rocq_alias discrete_cancelable]
 theorem discrete_cancelable {x : α} [Discrete α]
@@ -962,7 +962,7 @@ instance [CMRA β] : OFE (α -C> β) where
     symm h := dist_eqv.symm h
     trans h1 h2 := dist_eqv.trans h1 h2
   }
-  eq_dist' {_ _} := Hom.ext_iff.trans (eq_dist _)
+  eq_dist' {_ _} := Hom.ext_iff.trans eq_dist
   dist_lt := dist_lt
 
 @[rocq_alias cmra_morphism_id]
@@ -1683,7 +1683,7 @@ instance instCmraDistreteProd [CMRA.Discrete α] [CMRA.Discrete β] : CMRA.Discr
 @[rocq_alias pair_core_id]
 instance instCoreIdPair {x : α} {y : β} [CMRA.CoreId x] [CMRA.CoreId y] : CMRA.CoreId (α := α × β) ⟨x, y⟩ where
   core_id := by
-    refine ((OFE.eq_dist _).mpr (fun _ => ?_))
+    refine (OFE.eq_dist_2 (fun _ => ?_))
     simp only [CMRA.pcore, pcore]
     haveI : NonExpansive (fun b : β => some (x, b)) := ⟨fun _ _ _ H => some_dist_some.mpr (dist_prod_ext .rfl H)⟩
     haveI : NonExpansive ((fun a : α => (CMRA.pcore y).bind fun b : β => pure (a, b))) :=
