Iris/Iris/Algebra/COFESolver.lean
@@ -59,7 +59,7 @@ def down (k : Nat) : A F (k+1) -n> A F k := (updown F k).2
 @[rocq_alias solver.gf]
 theorem down_up : ∀ {k} x, down F k (up F k x) = x
   | 0, ⟨()⟩ => rfl
-  | _+1, x => (OFE.eq_dist _).mpr fun _ => (map_comp _ _ _ _ _).dist.symm.trans <|
+  | _+1, x => OFE.eq_dist_2 fun _ => (map_comp _ _ _ _ _).dist.symm.trans <|
     Dist.trans
       (map_ne.ne (fun y => (down_up y).dist) (fun y => (down_up y).dist) x)
       (map_id _).dist
@@ -87,7 +87,7 @@ instance : OFE (Tower F) where
     symm h _ := dist_eqv.symm (h _)
     trans h1 h2 _ := dist_eqv.trans (h1 _) (h2 _)
   }
-  eq_dist' {_ _} := by rw [Tower.ext_iff, funext_iff]; simpa only [eq_dist _] using forall_comm
+  eq_dist' {_ _} := by rw [Tower.ext_iff, funext_iff]; simpa only [eq_dist (SI:=_)] using forall_comm
   dist_lt h1 h2 _ := dist_lt (h1 _) h2
 
 #rocq_ignore solver.tower_equiv "Included in OFE (Tower F) instance"
@@ -102,7 +102,7 @@ def towerChain (c : Chain (SI := Nat) (Tower F)) (k : Nat) : Chain (A F k) where
 instance : COFE (Tower F) where
   compl c := by
     refine ⟨fun k => compl ⟨fun i => c.1 i k, fun h => c.cauchy h k⟩, ?_⟩
-    refine (OFE.eq_dist _).mpr (fun n => ?_)
+    refine OFE.eq_dist_2 (fun n => ?_)
     refine ((down ..).ne.1 conv_compl).trans <| .trans ?_ conv_compl.symm
     exact (c.chain n).down.dist
   conv_compl _ := conv_compl
@@ -212,7 +212,7 @@ protected def Tower.embed (k) : A F k -n> Tower F := by
 @[rocq_alias solver.embed_f]
 theorem Tower.embed_up (x : A F k) :
     Tower.embed (k+1) (up F k x) = Tower.embed k x := by
-  refine (OFE.eq_dist _).mpr (fun (n : Nat) i => ?_)
+  refine OFE.eq_dist_2 (fun (n : Nat) i => ?_)
   dsimp [Tower.embed, embed]; split <;> rename_i h₁
   · simp [Nat.le_of_succ_le h₁]
     suffices ∀ a b (e₁ : k + 1 + a = i) (e₂ : k+b = i),
@@ -271,7 +271,7 @@ def unfoldChain (X : Tower F) : Chain (F (Tower F) (Tower F)) where
 def Tower.isoAux : OFE.Iso (F (Tower F) (Tower F)) (Tower F) where
   hom.f X := {
     val n := (down F n).comp (map (Tower.embed _) (Tower.proj _)) X
-    down {n} := (OFE.eq_dist _).mpr fun m => (down ..).ne.1 <|
+    down {n} := OFE.eq_dist_2 fun m => (down ..).ne.1 <|
       (map_comp _ _ _ _ _).dist.symm.trans <|
         map_ne.ne (fun Y => (Tower.embed_up Y).dist) (fun Y => Y.down.dist) _
   }
@@ -280,7 +280,7 @@ def Tower.isoAux : OFE.Iso (F (Tower F) (Tower F)) (Tower F) where
   inv.ne.1 n _ _ h := by
     refine conv_compl.trans <| .trans ?_ conv_compl.symm
     exact (map ..).ne.1 (h (n+1))
-  hom_inv {X} := (OFE.eq_dist _).mpr fun n => by
+  hom_inv {X} := OFE.eq_dist_2 fun n => by
     intro k
     refine ((down ..).ne.1 (.trans ?_ (X.downN n).dist)).trans X.down.dist
     refine ((map ..).ne.1 (conv_compl.trans
@@ -309,7 +309,7 @@ def Tower.isoAux : OFE.Iso (F (Tower F) (Tower F)) (Tower F) where
         refine (map_comp _ _ _ _ _).dist.trans <|
           (ih (Nat.succ.inj e) _).trans (congrArg (fun a => (downN ..) a) ?_).dist
         exact (down_eqToHom _).symm
-  inv_hom := (OFE.eq_dist _).mpr fun n => by
+  inv_hom := OFE.eq_dist_2 fun n => by
     refine (conv_compl' n.le_succ).trans ?_
     dsimp [unfoldChain]; rw [down]
     refine ((map_comp _ _ _ _ _).trans
