Iris/Iris/Algebra/Csum.lean
@@ -53,7 +53,7 @@ instance [OFE α] [OFE β] : OFE (Csum α β) where
   Dist := Csum.Dist
   dist_eqv := dist_eqv
   eq_dist' {x y} := by
-    cases x <;> cases y <;> simp [Csum.Dist, (eq_dist _)]
+    cases x <;> cases y <;> simp [Csum.Dist, eq_dist (SI:=_)]
   dist_lt {n x y m} hn hlt := by
     cases x <;> cases y <;> first | exact OFE.Dist.lt hn hlt | exact hn.elim | trivial
 
