Iris/Iris/Algebra/Heap.lean
@@ -11,6 +11,7 @@ public import Iris.Std.Set
 public import Iris.Std.PartialMap
 
 @[expose] public section
+local stepindex Nat
 
 open Iris Std
 
@@ -20,13 +21,12 @@ open OFE
 
 namespace PartialMap
 
-local stepindex Nat
 instance instOFE [LawfulPartialMap M K] [OFE V] : OFE (M V) where
   Dist n s0 s1 := get? s0 ≡{n}≡ get? s1
   dist_eqv     := ⟨fun _ => .of_eq rfl, (·.symm), (·.trans ·)⟩
   eq_dist' {s0 s1} := by
     rw [← LawfulPartialMap.equiv_iff_eq]
-    exact ⟨fun h n k => Dist.of_eq (h k), fun h k => (eq_dist Nat).mpr fun n => h n k⟩
+    exact ⟨fun h n k => Dist.of_eq (h k), fun h k => eq_dist_2 fun n => h n k⟩
   dist_lt      := dist_lt
 
 @[simp] def toMap [LawfulPartialMap M K] [OFE V] : (M V) -n> (K → Option V) where
@@ -47,7 +47,7 @@ instance [LawfulPartialMap M K] [OFE V] (k : K) : NonExpansive₂ (insert · k �
     · simp [get?_insert_ne h, Hv k']
 
 theorem eqv_of_Equiv [OFE V] [LawfulPartialMap M K] {t1 t2 : M V} (H : PartialMap.equiv t1 t2) : t1 = t2 :=
-  (eq_dist Nat).mpr fun _ k => Dist.of_eq (H k)
+  eq_dist_2 fun _ k => Dist.of_eq (H k)
 
 instance [LawfulPartialMap M K] [OFE V] (op : K → V → V → V) [∀ k, NonExpansive₂ (op k)] :
     NonExpansive₂ (merge (M := M) op) where
@@ -63,8 +63,6 @@ theorem chain_get [LawfulPartialMap M K] [OFE V] (k : K) (c : Chain (M V)) :
 
 end PartialMap
 
-local stepindex Nat
-
 instance Heap.instCOFE [LawfulPartialMap M K] [COFE V] : COFE (M V) where
   compl c := bindAlter (fun _ => COFE.compl <| c.map ⟨_, PartialMap.get?_ne ·⟩) (c 0)
   conv_compl {_ c} k := by
@@ -77,13 +75,13 @@ instance Heap.instCOFE [LawfulPartialMap M K] [COFE V] : COFE (M V) where
   lbcompl_ne := (·.elim)
 
 instance instDiscreteHeap [LawfulPartialMap M K] [OFE V] [Discrete V] : Discrete (M V) where
-  discrete_0 h := (OFE.eq_dist Nat).mpr <| by
+  discrete_0 h := OFE.eq_dist_2 <| by
     intro _ k
     exact (Discrete.discrete_0 (h k)).dist
 
 instance instDiscreteESingleton [LawfulPartialMap M K] [DecidableEq K] [OFE V] {v : V}
     [ha : DiscreteE v] {k : K} : DiscreteE (PartialMap.singleton (M := M) k v) where
-  discrete {y} h := (OFE.eq_dist Nat).mpr <| by
+  discrete {y} h := OFE.eq_dist_2 <| by
     intro n k'
     by_cases hh : k = k'
     · simp only [LawfulPartialMap.get?_singleton, hh, ↓reduceIte]
@@ -94,7 +92,7 @@ instance instDiscreteESingleton [LawfulPartialMap M K] [DecidableEq K] [OFE V] {
       simp [LawfulPartialMap.get?_singleton, hh, ↓reduceIte]
 
 instance instDiscreteEEmpty [LawfulPartialMap M K] [OFE V] : DiscreteE (∅ : M V) where
-  discrete {y} h := (OFE.eq_dist Nat).mpr <| by
+  discrete {y} h := OFE.eq_dist_2 <| by
     intro n k
     simp only [LawfulPartialMap.get?_empty]
     refine (DiscreteE.discrete (.trans ?_ (h k))).dist
@@ -125,7 +123,6 @@ variable [LawfulPartialMap M K] [CMRA V]
 @[simp] def valid (s : M V) : Prop := ∀ k, ✓ get? s k
 @[simp] def validN (n : Nat) (s : M V) : Prop := ∀ k, ✓{n} get? s k
 
-local stepindex Nat
 theorem lookup_incN {n} {m1 m2 : M V} :
     (∃ (z : M V), m2 ≡{n}≡ op m1 z) ↔
     ∀ i, (∃ z, (get? m2 i) ≡{n}≡ (get? m1 i) • z) := by
@@ -151,7 +148,7 @@ theorem lookup_inc {m1 m2 : M V} :
     cases get? m1 i <;> cases get? z i <;> simp
   · obtain ⟨f, Hf⟩ := Classical.axiomOfChoice H
     exists bindAlter (fun k _ => f k) m2
-    refine (OFE.eq_dist Nat).mpr fun n i => ((Hf i).trans ?_).dist
+    refine OFE.eq_dist_2 fun n i => ((Hf i).trans ?_).dist
     specialize Hf i; revert Hf
     simp [CMRA.op, optionOp, get?_merge, get?_bindAlter]
     cases get? m2 i <;> cases get? m1 i <;> cases f i <;> simp <;>
@@ -186,15 +183,15 @@ instance instStoreCMRA : CMRA (M V) where
     specialize H k; revert H
     simp only [op, get?_merge, Option.merge]
     cases get? x1 k <;> cases get? x2 k <;> simp [optionOp, CMRA.op]
-  assoc {x y z} := (eq_dist Nat).mpr fun _ k => by
+  assoc {x y z} := eq_dist_2 fun _ k => by
     simp only [op, get?_merge]
     cases get? x k <;> cases get? y k <;> cases get? z k <;> simp
     exact assoc.dist
-  comm {x y} := (eq_dist Nat).mpr fun _ k => by
+  comm {x y} := eq_dist_2 fun _ k => by
     simp [op, get?_merge]
     cases get? x k <;> cases get? y k <;> simp
     exact comm.dist
-  pcore_op_left {x cx} H := (eq_dist Nat).mpr fun _ k => by
+  pcore_op_left {x cx} H := eq_dist_2 fun _ k => by
     simp only [← Option.getD_some (a := cx) (b := cx), op, get?_merge]
     cases Hcx : get? cx k <;> cases hx : get? x k <;>
       simp <;>
@@ -203,7 +200,7 @@ instance instStoreCMRA : CMRA (M V) where
       cases Hcx
     · refine (pcore_op_left ?_).dist
       simp [← Hcx, ← H, get?_bindAlter, hx]
-  pcore_idem {x cx} H := (eq_dist Nat).mpr <| by
+  pcore_idem {x cx} H := eq_dist_2 <| by
     simp only [pcore, Option.some.injEq] at H
     simp only [pcore, ← H]
     intro n k
@@ -219,7 +216,7 @@ instance instStoreCMRA : CMRA (M V) where
       simp only [pcore, Option.some.injEq, op, exists_eq_left']
       rcases this with ⟨z', Hz'⟩
       exists z'
-      refine Hz'.trans ((OFE.eq_dist Nat).mpr fun n i => ?_)
+      refine Hz'.trans (OFE.eq_dist_2 fun n i => ?_)
       cases get? z' i <;> cases get? x i <;> simp_all
     refine lookup_inc.mpr (fun i => ?_)
     obtain ⟨v', Hv'⟩ : (core (get? x i)) ≼ (core (get? y i))  := by
@@ -239,7 +236,7 @@ instance instStoreCMRA : CMRA (M V) where
     exists bindAlter (fun k (_ : V) => extendF k |>.fst) y1
     exists bindAlter (fun k (_ : V) => extendF k |>.snd.fst) y2
     simp [op]
-    refine ⟨(eq_dist Nat).mpr fun _ i => ?_, fun i => ?_, fun i => ?_⟩
+    refine ⟨eq_dist_2 fun _ i => ?_, fun i => ?_, fun i => ?_⟩
     all_goals rcases hF : extendF i with ⟨z1, z2, Hm, Hz1, Hz2⟩
     · refine Hm.dist.trans ?_
       simp [get?_merge, CMRA.op, optionOp, Option.merge, get?_bindAlter]
@@ -265,8 +262,8 @@ instance instStoreCMRA : CMRA (M V) where
 instance instStoreUCMRA : UCMRA (M V) where
   unit := unit
   unit_valid := by simp [CMRA.Valid, get?_empty]
-  unit_left_id := (OFE.eq_dist Nat).mpr fun _ k => by simp [CMRA.op, get?_merge, get?_empty]
-  pcore_unit := (OFE.eq_dist Nat).mpr fun _ => by
+  unit_left_id := OFE.eq_dist_2 fun _ k => by simp [CMRA.op, get?_merge, get?_empty]
+  pcore_unit := OFE.eq_dist_2 fun _ => by
     refine OFE.some_dist_some.mpr fun k => ?_
     simp [get?_bindAlter, get?_empty]
 
@@ -352,7 +349,7 @@ theorem insert_eq_singleton_op_singleton [IsoFunMap M K] {m : M V} (Hemp : get? 
     insert m i x = singleton i x • m :=
   IsoFunMap.ext (insert_equiv_singleton_op_singleton Hemp)
 
-theorem core_empty : core (∅ : M V) = ∅ := (OFE.eq_dist Nat).mpr <| by
+theorem core_empty : core (∅ : M V) = ∅ := OFE.eq_dist_2 <| by
   intro n k
   simp [core, CMRA.pcore, get?_empty, get?_bindAlter]
 
@@ -369,7 +366,7 @@ theorem singleton_core_eq [IsoFunMap M K] {i : K} {x : V} {cx} (Hpcore : CMRA.pc
 
 open Classical in
 theorem singleton_core_eqv {i : K} {x : V} {cx} (Hpcore : CMRA.pcore x = some cx) :
-    core (singleton i x : M V) = singleton i cx := (OFE.eq_dist Nat).mpr <| by
+    core (singleton i x : M V) = singleton i cx := OFE.eq_dist_2 <| by
   intro n k
   simp [core, CMRA.pcore, get?_singleton, get?_bindAlter]
   split <;> first | exact Hpcore.dist | trivial
@@ -394,7 +391,7 @@ theorem singleton_op_singleton_eq [IsoFunMap M K] {i : K} {x y : V} :
   IsoFunMap.ext singleton_op_singleton
 
 instance {m : M V} [I : ∀ x : V, CoreId x] : CoreId m where
-  core_id := (OFE.eq_dist Nat).mpr fun _ => by
+  core_id := OFE.eq_dist_2 fun _ => by
     refine OFE.some_dist_some.mpr fun k => ?_
     rw [get?_bindAlter]
     cases get? m k <;> simp
@@ -402,7 +399,7 @@ instance {m : M V} [I : ∀ x : V, CoreId x] : CoreId m where
 
 open Classical in
 instance [CoreId (x : V)] : CoreId (singleton i x : M V) where
-  core_id := (OFE.eq_dist Nat).mpr fun _ => by
+  core_id := OFE.eq_dist_2 fun _ => by
     refine OFE.some_dist_some.mpr fun k => ?_
     simp [get?_bindAlter, get?_singleton]
     split <;> simp
@@ -453,7 +450,7 @@ theorem singleton_inc_iff {m : M V} :
       exists v
   · cases z
     · exists (PartialMap.delete m i)
-      refine (OFE.eq_dist Nat).mpr fun _ j => ?_
+      refine OFE.eq_dist_2 fun _ j => ?_
       simp [CMRA.op, get?_merge, get?_singleton, get?_delete]
       split
       · rename_i h
@@ -463,7 +460,7 @@ theorem singleton_inc_iff {m : M V} :
       · simp
     · rename_i z
       exists (PartialMap.insert m i z)
-      refine (OFE.eq_dist Nat).mpr fun _ j => ?_
+      refine OFE.eq_dist_2 fun _ j => ?_
       simp [CMRA.op, get?_merge, get?_singleton, get?_insert]
       split
       · rename_i h
@@ -472,7 +469,6 @@ theorem singleton_inc_iff {m : M V} :
         simp [CMRA.op]
       · simp
 
-local stepindex Nat
 theorem exclusive_singleton_inc_iff {m : M V} (He : Exclusive x) (Hv : ✓ m) :
     (singleton i x) ≼ m ↔ (get? m i = some x) := by
   refine singleton_inc_iff.trans ⟨fun ⟨y, Hy, Hxy⟩ => ?_, fun _ => ?_⟩
@@ -568,7 +564,9 @@ theorem inc_dom_inc {m1 m2 : M V} (Hinc : m1 ≼ m2) : Set.Included (dom m1) (do
     exact fun h => (OFE.not_none_eqv_some h).elim
 
 nonrec instance [HD : CMRA.Discrete V] [LawfulPartialMap M K] : Discrete (M V) where
-  discrete_0 {_ _} H := (OFE.eq_dist Nat).mpr fun _ k => (OFE.Discrete.discrete_0 (H k)).dist
+  discrete_0 {_ _} H := by
+    refine OFE.eq_dist_2 ?_
+    exact fun _ k => (OFE.Discrete.discrete_0 (H k)).dist
   discrete_valid {_} := (CMRA.Discrete.discrete_valid <| · ·)
 
 end Heap
@@ -581,7 +579,6 @@ namespace PartialMap
 
 def map (f : α → β) : H α → H β := PartialMap.bindAlter (fun _ a => some <| f a)
 
-local stepindex Nat
 instance [OFE α] [OFE β] {f : α → β} [hne : OFE.NonExpansive f] : OFE.NonExpansive (map H f) where
   ne := by
     simp only [OFE.Dist, Option.Forall₂, map, get?_bindAlter, Option.bind]
@@ -590,7 +587,7 @@ instance [OFE α] [OFE β] {f : α → β} [hne : OFE.NonExpansive f] : OFE.NonE
     apply OFE.NonExpansive.ne
 
 theorem map_id [OFE α] (a : H α) :
-    PartialMap.map H id a = a := (OFE.eq_dist Nat).mpr <| by
+    PartialMap.map H id a = a := OFE.eq_dist_2 <| by
   intro n x
   simp [PartialMap.map, get?_bindAlter, Option.bind]
   rcases get? a x <;> simp
@@ -606,7 +603,7 @@ theorem map_ne [OFE α] [OFE β] (f g : α -> β) {heq : f ≡{n}≡ g} : map H 
   exact heq _
 
 theorem map_compose [OFE α] [OFE β] [OFE γ] (f : α -> β) (g : β -> γ) m :
-    map H (g.comp f) m = map H g (map H f m) := (OFE.eq_dist Nat).mpr <| by
+    map H (g.comp f) m = map H g (map H f m) := OFE.eq_dist_2 <| by
   intro n k
   simp [map, get?_bindAlter]
   cases get? m k <;> simp
@@ -621,7 +618,7 @@ def mapC [CMRA α] [CMRA β] (f : α -C> β) : CMRA.Hom (H α) (H β) where
     rw [get?_bindAlter]
     cases (get? x k) <;> simp
     apply CMRA.Hom.validN
-  pcore m := (OFE.eq_dist Nat).mpr <| by
+  pcore m := OFE.eq_dist_2 <| by
     intro _ x
     simp [map, get?_bindAlter]
     rcases get? m x with _|v <;> simp
@@ -630,7 +627,7 @@ def mapC [CMRA α] [CMRA β] (f : α -C> β) : CMRA.Hom (H α) (H β) where
       rfl
     rw [h]
     exact (CMRA.Hom.pcore f v).dist
-  op m1 m2 := (OFE.eq_dist Nat).mpr <| by
+  op m1 m2 := OFE.eq_dist_2 <| by
     intro _ k
     simp [CMRA.op, map, get?_bindAlter, get?_merge, Option.merge]
     cases get? m1 k <;> cases get? m2 k <;> simp
@@ -650,7 +647,7 @@ instance {F} [COFE.OFunctor F] : COFE.OFunctor (PartialMapOF H F) where
   map_id x := by
     refine .trans ?_ (map_id H x)
     exact congrArg (map H · x) (funext fun a => COFE.OFunctor.map_id a)
-  map_comp f g f' g' m := (OFE.eq_dist Nat).mpr <| by
+  map_comp f g f' g' m := OFE.eq_dist_2 <| by
     simp [mapO, map]
     intro n x
     simp [get?_bindAlter]
@@ -667,7 +664,7 @@ instance {F} [RFunctor F] : URFunctor (PartialMapOF H F) where
   map_id x := by
     refine .trans ?_ (map_id H x)
     exact congrArg (map H · x) (funext fun a => RFunctor.map_id a)
-  map_comp f g f' g' m := (OFE.eq_dist Nat).mpr <| by
+  map_comp f g f' g' m := OFE.eq_dist_2 <| by
     simp [mapC, map]
     intro n x
     simp [get?_bindAlter]
