Iris/Iris/Examples/IProp.lean
@@ -146,7 +146,7 @@ theorem wp_unfold (e : Expr) (Φ : Value → IProp GF) :
         ∀ s, @state_interp State _ _ s -∗
           ∃ e' s', ⌜@step _ _ Value _ (e, s) = (e', s') ⌝ ∗
           ▷ |==> (@state_interp _ _ _  s' ∗ wp e' Φ)) := by
-  exact (OFE.eq_dist _).mpr fun _n => (fixpoint_unfold (f := ⟨(@wp_F Expr State Value _ GF _),
+  exact OFE.eq_dist_2 fun _n => (fixpoint_unfold (f := ⟨(@wp_F Expr State Value _ GF _),
                                 @OFE.ne_of_contractive _ _ _ _ _ _ (@wp_F Expr State Value _ GF _) _⟩)).dist (SI := Nat) e Φ
 
 /- Now, we can derive some example proof rules. First let's prove a rule for pure deterministic steps: -/
