Iris/Iris/Instances/IProp/Instance.lean
@@ -171,14 +171,14 @@ def IProp.foldi : FF.api τ (IPre FF) -n> FF.api τ (IProp FF) :=
 
 @[rocq_alias inG_unfold_fold]
 theorem IProp.unfoldi_foldi (x : FF.api τ (IPre FF)) : unfoldi (foldi x) = x := by
-  refine (OFE.eq_dist _).mpr fun n => ?_
+  refine OFE.eq_dist_2 fun n => ?_
   refine .trans (OFunctor.map_comp (F := FF τ |>.fst) ..).symm.dist ?_
   refine .trans ?_ (OFunctor.map_id (F := FF τ |>.fst) x).dist
   apply OFunctor.map_ne.ne <;> intro _ <;> simp [IProp.unfold, IProp.fold]
 
 @[rocq_alias inG_fold_unfold]
 theorem IProp.foldi_unfoldi (x : FF.api τ (IProp FF)) : foldi (unfoldi x) = x := by
-  refine (OFE.eq_dist _).mpr fun n => ?_
+  refine OFE.eq_dist_2 fun n => ?_
   refine .trans (OFunctor.map_comp (F := FF τ |>.fst) ..).symm.dist ?_
   refine .trans ?_ (OFunctor.map_id (F := FF τ |>.fst) x).dist
   apply OFunctor.map_ne.ne <;> intro _ <;> simp [IProp.unfold, IProp.fold]
@@ -262,7 +262,7 @@ instance : OFE.NonExpansive (iSingleton F γ (GF := GF)) where
 
 @[rocq_alias iRes_singleton_op]
 theorem iSingleton_op (x y : F.ap (IProp GF)) : (iSingleton F γ x) • iSingleton F γ y = iSingleton F γ (x • y) := by
-  refine (OFE.eq_dist _).mpr fun n => ?_
+  refine OFE.eq_dist_2 fun n => ?_
   intro τ' γ'
   simp only [iSingleton]
   split
@@ -315,7 +315,7 @@ theorem unfoldi_bundle_coreId {a : F.ap (IProp GF)} [CMRA.CoreId a] :
 
 @[rocq_alias iRes_singleton_core_id]
 instance {a : F.ap (IProp GF)} [CMRA.CoreId a] : CMRA.CoreId (iSingleton F γ a) where
-  core_id := (OFE.eq_dist _).mpr fun n τ' γ' => by
+  core_id := OFE.eq_dist_2 fun n τ' γ' => by
     show CMRA.core ((iSingleton F γ a τ').car γ') ≡{n}≡ (iSingleton F γ a τ').car γ'
     simp only [iSingleton]
     split
@@ -447,7 +447,7 @@ theorem iSingleton_op_validN_at_γ {a : F.ap (IProp GF)} (Hv : ✓{n} mf) :
 instance iSingleton_discreteE {v : F.ap (IProp GF)} [inst : OFE.DiscreteE v] :
     OFE.DiscreteE (iSingleton F γ v) where
   discrete {w} H := by
-    refine (OFE.eq_dist _).mpr fun n τ => ?_
+    refine OFE.eq_dist_2 fun n τ => ?_
     simp only [iSingleton] at ⊢
     split
     next h =>
