Iris/Iris/Instances/UPred/Instance.lean
@@ -285,7 +285,7 @@ instance : BI (UPred M) where
   entails_refl := uPred_entails_preorder.le_refl _
   entails_trans := uPred_entails_preorder.le_trans _ _ _
   equiv_iff {_ _} := by
-    rw [(OFE.eq_dist _)]
+    rw [OFE.eq_dist]
     constructor <;> intro HE
     · exact ⟨fun n ⟨x, Hv⟩ H => (HE n n x .refl Hv).mp H,
              fun n ⟨x, Hv⟩ H => (HE n n x .refl Hv).mpr H⟩
