Iris/Iris/ProgramLogic/WeakestPre.lean
@@ -128,7 +128,7 @@ section Wp
 @[rocq_alias wp_unfold]
 theorem wp_unfold {s E} {e : Expr} {Φ : Val → IProp GF} :
     WP e @ s ; E {{ Φ }} ⊣⊢ wp.pre s (Wp.wp (PROP := IProp GF) s) E e Φ :=
-  BI.equiv_iff.1 <| (OFE.eq_dist _).mpr <|
+  BI.equiv_iff.1 <| OFE.eq_dist_2 <|
     fun _n => (fixpoint_unfold (f := (wp.pre s).toContractiveHom)).dist (SI := Nat) E e Φ
 
 @[rocq_alias wp_ne]
